{
 "cells": [
  {
   "cell_type": "markdown",
   "metadata": {},
   "source": [
    "# MAE598 HW 2\n",
    "\n",
    "Name: Zachary Poit\n",
    "\n",
    "### Question 1: \n",
    "\n",
    "Function: $ 2 x_1^2 - 4 x_1 x_2 + 1.5 x_2^2 + x_2$\n",
    "\n",
    "$ \\nabla f = \n",
    "\\begin{bmatrix}\n",
    "4 (x_1 - x_2) \\\\\n",
    "-4 x_1 + 3 x_2 + 1 \\\\\n",
    "\\end{bmatrix}$ \n",
    "\n",
    "$ H_f = \n",
    "\\begin{bmatrix}\n",
    "4 & -4 \\\\\n",
    "-4 & 3 \\\\\n",
    "\\end{bmatrix}$\n",
    "\n",
    "$ \\left| H - I \\lambda \\right| = \\begin{bmatrix}\n",
    "4- \\lambda & -4 \\\\\n",
    "-4 & 3 -\\lambda\\\\\n",
    "\\end{bmatrix} = \\lambda^2 - 7 \\lambda -4$ \n",
    "\n",
    "$\\lambda_{1,2} = \\frac{7 \\pm \\sqrt{65}}{2}$ \n",
    "\n",
    "The eigen values are not all positive or all negitive or zero so the Hessian is a indefinite matrix. So we have a saddle!\n",
    "\n",
    "Taylor expansion at saddle point (Gradient is zero): $ f(x_1,x_2) = f(1,1) + \\frac{1}{2} \\begin{bmatrix}\n",
    "x_1 - 1 & x_2 - 1\\\\\n",
    "\\end{bmatrix}\\begin{bmatrix}\n",
    "4 & -4 \\\\\n",
    "-4 & 3 \\\\\n",
    "\\end{bmatrix}\\begin{bmatrix}\n",
    "x_1 - 1 \\\\\n",
    " x_2 - 1\\\\\n",
    "\\end{bmatrix}$\n",
    "\n",
    "$ f(x_1,x_2) = f(1,1) + \\frac{1}{2} \\begin{bmatrix}\n",
    "\\partial x_1 & \\partial x_2\\\\\n",
    "\\end{bmatrix}\\begin{bmatrix}\n",
    "4 & -4 \\\\\n",
    "-4 & 3 \\\\\n",
    "\\end{bmatrix}\\begin{bmatrix}\n",
    "\\partial x_1 \\\\\n",
    "\\partial x_2\\\\\n",
    "\\end{bmatrix}$\n",
    "\n",
    "$ f(x_1,x_2) = f(1,1) + \\frac{1}{2} \\left( 4 \\partial x_1^2 - 8 \\partial x_1 \\partial x_2 + 3 \\partial x_2^2\\right) $\n",
    "\n",
    "$ f(x_1,x_2) = f(1,1) + \n",
    "\n",
    "Factor this to put it in form $ f(x_1,x_2) = f(1,1) + \\left( a \\partial x_1 - b \\partial x_2 \\right)\\left( c \\partial x_1 - d \\partial x_2 \\right)$\n",
    "\n",
    "We get the following equations:\n",
    "\n",
    "$ ac = 2$\n",
    "\n",
    "$bd = 1.5$\n",
    "\n",
    "$ad + bc = 4$\n",
    "\n",
    "If we set $ a = 1 $ then, $ c = 2 $, $ d = 1 $, and $ b = \\frac{3}{2}$\n",
    "\n",
    "$ f(x_1,x_2) = f(1,1) + \\left( \\partial x_1 - \\frac{3}{2} \\partial x_2 \\right)\\left( 2\\partial x_1 - \\partial x_2 \\right)$\n",
    "\n",
    "$ \\left( \\partial x_1 - \\frac{3}{2} \\partial x_2 \\right)\\left( 2\\partial x_1 - \\partial x_2 \\right) < 0$ \n",
    "\n",
    "Two cases for the directions: \n",
    "\n",
    "Case 1: $ \\left( \\partial x_1 - \\frac{3}{2} \\partial x_2 \\right) > 0$ and $\\left( 2\\partial x_1 - \\partial x_2 \\right) < 0$ \n",
    "\n",
    "Case 2: $ \\left( \\partial x_1 - \\frac{3}{2} \\partial x_2 \\right) < 0$ and $\\left( 2\\partial x_1 - \\partial x_2 \\right) > 0$ \n"
   ]
  },
  {
   "cell_type": "markdown",
   "metadata": {},
   "source": [
    "### Question 2: \n",
    "\n",
    "#### Part a:\n",
    "\n",
    "Step 1: solve the problem with just multivarite Calculus concepts:\n",
    "\n",
    "Reference point:\n",
    "\n",
    "$ P = (-1,0,1)^T $\n",
    "\n",
    "A point on the plane:\n",
    "\n",
    "$ Q = (1,0,0)^T $\n",
    "\n",
    "vector from Q to P:\n",
    "\n",
    "$ v = P - Q = (-2, 0, 1)^T $\n",
    "\n",
    "Normal vector: \n",
    "\n",
    "$ \\hat{n} = \\frac{(1,2,3)^T}{\\sqrt{1^2 + 2^2 + 3^2}} = \\left(\\frac{1}{\\sqrt{14}},\\frac{2}{\\sqrt{14}},\\frac{3}{\\sqrt{14}}\\right)^T$\n",
    "\n",
    "Find distance shortest distance between reference point and plane\n",
    "\n",
    "$D = v^T \\hat{n} = (-2, 0, 1) \\left(\\frac{1}{\\sqrt{14}},\\frac{2}{\\sqrt{14}},\\frac{3}{\\sqrt{14}}\\right)^T = \\frac{1}{\\sqrt{14}}$\n",
    "\n",
    "Subtract that distance times normal vector from reference point to get answer!\n",
    "\n",
    "$ A = P - D*\\hat{n} = (-1,0,1)^T - \\left(\\frac{1}{14},\\frac{2}{14},\\frac{3}{14}\\right)^T = \\left(-\\frac{15}{14},-\\frac{1}{7},\\frac{11}{14}\\right)^T$\n",
    "\n",
    "Step 2: Solve the problem using optimization:\n",
    "\n",
    "Distance from any point to the reference point is the 2 - norm. \n",
    "\n",
    "$ D = \\sqrt{(x_1 + 1)^2 + x_2^2 + (x_3 - 1)^2} $\n",
    "\n",
    "This is a convex function because the term inside the square root is a convex function. The square root of a convex function is also a convex function. \n",
    "\n",
    "There is also $x_1 + 2x_2 + 3x_3 = 1$ which is a convex set (convex plane) which constrains $x_1, x_2, x_3$ to the plane.\n",
    "\n",
    "To make it unconstrained optimization problem, substitute into the convex function. \n",
    "\n",
    "$ D = \\sqrt{(1 - 2x_2 - 3x_3 + 1)^2 + x_2^2 + (x_3 - 1)^2} $\n",
    "\n",
    "#### Part B:"
   ]
  },
  {
   "cell_type": "code",
   "execution_count": null,
   "metadata": {},
   "outputs": [],
   "source": []
  },
  {
   "cell_type": "markdown",
   "metadata": {},
   "source": [
    "### Question 3:\n",
    "\n",
    "Define function $f(x) = a^T x = a_1 x_1 + a_2 x_2 + ... + a_n x_n$\n",
    "\n",
    "$\\nabla f = a$\n",
    "\n",
    "$H_f = 0_{nxn}$\n",
    "\n",
    "Since the Hessian is Positive semi definite, the function is convex. (It is also negitive semi definite, so also concave)\n",
    "\n",
    "if $f(x)$ is convex then $ S_1 = \\{ x \\in \\R^n | f(x) \\leq c \\}$ is convex set. This is a half hyper space\n",
    "\n",
    "The other half hyper space $ S_2 = \\{ x \\in \\R^n | f(x) \\geq c \\}$ is also convex. \n",
    "\n",
    "The intersection of these two half hyper spaces gives us the set $ S_1 \\cap S_2 = S_3 = \\{ x \\in \\R^n | f(x) = c \\}$ which is the hyper plane \n",
    "\n",
    "The intersection of two convex sets are convex."
   ]
  }
 ],
 "metadata": {
  "kernelspec": {
   "display_name": "Python 3.10.4 64-bit",
   "language": "python",
   "name": "python3"
  },
  "language_info": {
   "name": "python",
   "version": "3.10.4"
  },
  "orig_nbformat": 4,
  "vscode": {
   "interpreter": {
    "hash": "916dbcbb3f70747c44a77c7bcd40155683ae19c65e1c03b4aa3499c5328201f1"
   }
  }
 },
 "nbformat": 4,
 "nbformat_minor": 2
}
